examples/load_test.v
@@ -2,7 +2,7 @@ Require Import isla.base.
 Require Import isla.opsem.
 Require Import isla.automation.
 Require Import isla.instructions.load.
-Require Import isla.examples.sys_regs.
+Require Import isla.sys_regs.
 
 Definition spec `{!islaG Σ} `{!threadG} a : iProp Σ :=
   ∃ (vold : bv 64),
